Lookup

theories/arraylist.v
@@ -6,3 +6,27 @@ From Coq Require Export Lia.
 From Coq Require Export Lists.List.
 Export ListNotations.
 From Coq Require Export Permutation.
+
+
+
+
+
+
+Fixpoint lookup (i : nat) (l : list nat) := 
+    match l with
+    | [] => 0
+    | h :: t => if i <=? 0 then h else lookup (i-1) t
+    end.
+   
+
+Example lookup_example1 :
+    lookup 3 [2;3;4;5;1;2] = 5.
+Proof. simpl. reflexivity. Qed.
+
+Example lookup_example_empty_list :
+    lookup 3 [] = 0.
+Proof. simpl. reflexivity. Qed.
+
+Example lookup_example_higher_than_list :
+    lookup 10 [2;3;4;5;1;2] = 0.
+Proof. simpl. reflexivity. Qed.
